\begin{eqnarray}
J(1,1)&=&\begin{bmatrix}
- 20\cdot \sin(\theta_1 + \theta_2) - 20\cdot \sin(\theta_1)\\ 
\end{bmatrix}
 \nonumber \\J(1,2)&=&\begin{bmatrix}
-20\cdot \sin(\theta_1 + \theta_2)\\ 
\end{bmatrix}
 \nonumber \\J(2,1)&=&\begin{bmatrix}
20\cdot \cos(\theta_1 + \theta_2) + 20\cdot \cos(\theta_1)\\ 
\end{bmatrix}
 \nonumber \\J(2,2)&=&\begin{bmatrix}
20\cdot \cos(\theta_1 + \theta_2)\\ 
\end{bmatrix}
 \nonumber \\J(3,1)&=&\begin{bmatrix}
0\\ 
\end{bmatrix}
 \nonumber \\J(3,2)&=&\begin{bmatrix}
0\\ 
\end{bmatrix}
 \nonumber \\J(4,1)&=&\begin{bmatrix}
0\\ 
\end{bmatrix}
 \nonumber \\J(4,2)&=&\begin{bmatrix}
0\\ 
\end{bmatrix}
 \nonumber \\J(5,1)&=&\begin{bmatrix}
0\\ 
\end{bmatrix}
 \nonumber \\J(5,2)&=&\begin{bmatrix}
0\\ 
\end{bmatrix}
 \nonumber \\J(6,1)&=&\begin{bmatrix}
1\\ 
\end{bmatrix}
 \nonumber \\J(6,2)&=&\begin{bmatrix}
1\\ 
\end{bmatrix}
 \nonumber\end{eqnarray}
