\begin{eqnarray}
J(1,1)&=&\begin{bmatrix}
5\cdot \cos(\theta_1)\cdot \sin(\theta_2) - 4\cdot \sin(\theta_1) + 4\cdot \cos(\theta_1)\cdot \cos(\theta_2)\cdot \sin(\theta_3) + 4\cdot \cos(\theta_1)\cdot \cos(\theta_3)\cdot \sin(\theta_2)\\ 
\end{bmatrix}
 \nonumber \\J(1,2)&=&\begin{bmatrix}
\sin(\theta_1)\cdot (4\cdot \cos(\theta_2 + \theta_3) + 5\cdot \cos(\theta_2))\\ 
\end{bmatrix}
 \nonumber \\J(1,3)&=&\begin{bmatrix}
4\cdot \cos(\theta_2 + \theta_3)\cdot \sin(\theta_1)\\ 
\end{bmatrix}
 \nonumber \\J(2,1)&=&\begin{bmatrix}
4\cdot \cos(\theta_1) + 5\cdot \sin(\theta_1)\cdot \sin(\theta_2) + 4\cdot \cos(\theta_2)\cdot \sin(\theta_1)\cdot \sin(\theta_3) + 4\cdot \cos(\theta_3)\cdot \sin(\theta_1)\cdot \sin(\theta_2)\\ 
\end{bmatrix}
 \nonumber \\J(2,2)&=&\begin{bmatrix}
-\cos(\theta_1)\cdot (4\cdot \cos(\theta_2 + \theta_3) + 5\cdot \cos(\theta_2))\\ 
\end{bmatrix}
 \nonumber \\J(2,3)&=&\begin{bmatrix}
-4\cdot \cos(\theta_2 + \theta_3)\cdot \cos(\theta_1)\\ 
\end{bmatrix}
 \nonumber \\J(3,1)&=&\begin{bmatrix}
0\\ 
\end{bmatrix}
 \nonumber \\J(3,2)&=&\begin{bmatrix}
- 4\cdot \sin(\theta_2 + \theta_3) - 5\cdot \sin(\theta_2)\\ 
\end{bmatrix}
 \nonumber \\J(3,3)&=&\begin{bmatrix}
-4\cdot \sin(\theta_2 + \theta_3)\\ 
\end{bmatrix}
 \nonumber \\J(4,1)&=&\begin{bmatrix}
0\\ 
\end{bmatrix}
 \nonumber \\J(4,2)&=&\begin{bmatrix}
\cos(\theta_1)\\ 
\end{bmatrix}
 \nonumber \\J(4,3)&=&\begin{bmatrix}
\cos(\theta_1)\\ 
\end{bmatrix}
 \nonumber \\J(5,1)&=&\begin{bmatrix}
0\\ 
\end{bmatrix}
 \nonumber \\J(5,2)&=&\begin{bmatrix}
\sin(\theta_1)\\ 
\end{bmatrix}
 \nonumber \\J(5,3)&=&\begin{bmatrix}
\sin(\theta_1)\\ 
\end{bmatrix}
 \nonumber \\J(6,1)&=&\begin{bmatrix}
1\\ 
\end{bmatrix}
 \nonumber \\J(6,2)&=&\begin{bmatrix}
0\\ 
\end{bmatrix}
 \nonumber \\J(6,3)&=&\begin{bmatrix}
0\\ 
\end{bmatrix}
 \nonumber\end{eqnarray}
